concurrency/bst_conc_nblocking_spec.v
@@ -106,6 +106,209 @@ Definition Gprog : funspecs :=
     spawn_spec;
     main_spec 
   ]).
+  
+  Lemma split_non_bot_share sh :
+   (sh <> Share.bot) ->
+  exists sh1, exists sh2,
+     (sh1 <> Share.bot) /\
+     (sh2 <> Share.bot) /\
+    sepalg.join sh1 sh2 sh.
+Proof.
+  intros.
+  destruct (Share.split sh) as (sh1, sh2) eqn: Hsplit.
+  exists sh1, sh2; split; [|split]; auto.
+  intro X. contradiction H. apply (Share.split_nontrivial sh1 sh2 sh) . auto. left. auto.
+  intro X. contradiction H. apply (Share.split_nontrivial sh1 sh2 sh) . auto. right. auto.
+  apply split_join; auto.
+Qed.
+   
+Lemma in_tree_split: forall g_in range p g, in_tree g_in range p g |-- in_tree g_in range p g * in_tree g_in range p g.
+Proof.
+intros. unfold in_tree. Intro sh. assert_PROP ( sh <> Share.bot).  { unfold ghost_part. sep_apply (own_valid (RA := ref_PCM (map_PCM (A:= gname ) )) g ((Some (sh, ghosts.singleton  (P:= prod_PCM range_ghost (discrete_PCM val)) g_in (range, p)), None) ) compcert_rmaps.RML.R.NoneP). entailer!. inv H. simpl in H0. contradiction. } apply split_non_bot_share in H. destruct H as ( sh1 & sh2 & H1 & H2 & H).
+Exists sh1 sh2. rewrite <- (ghost_part_join (P:= map_PCM (A:= gname ) ) sh1 sh2 sh  (ghosts.singleton  (P:= prod_PCM range_ghost (discrete_PCM val)) g_in (range, p))  (ghosts.singleton  (P:= prod_PCM range_ghost (discrete_PCM val))  g_in (range, p))).
+cancel. auto. { unfold sepalg.join. hnf. intro. hnf. simpl. destruct (ghosts.singleton (P:= prod_PCM range_ghost (discrete_PCM val)) g_in (range, p) k). 
+  -  apply psepalg.lower_Some. unfold sepalg.join. hnf. split; hnf. rewrite merge_self;auto. split;auto.
+  - apply psepalg.lower_None1. 
+  } auto. auto. 
+ Qed.
+ 
+Notation empty := (@empty coPset _).
+Notation top := (@top coPset _).
+
+Definition node_data (info: option ghost_info) g  tp lp rp (range:number * number)  :=  
+(match info with Some data =>  EX sh, !!(readable_share sh) &&  data_at sh t_struct_tree (Vint (Int.repr data.1.1.1),(data.1.1.2,(lp,rp))) tp * in_tree  data.1.2 ( fst range, Finite_Integer (data.1.1.1)) lp g * in_tree data.2 ( Finite_Integer (data.1.1.1), snd range) rp g | None => !!(tp = nullval) && emp end).
+ 
+
+Definition node_information (info: option ghost_info) range g g_current tp lp rp np  :=  bst.bst_conc_nblocking_spec.atomic_ptr_at Ews tp np * ghost_master1 (ORD := range_order)  (range, info) g_current * 
+node_data info g tp lp rp range.
+
+Lemma node_data_split : forall (info: option ghost_info) g  tp lp rp (range:number *number), node_data info g tp lp rp range |-- node_data info g tp lp rp range * node_data info g tp lp rp range.
+Proof.
+intros.
+unfold node_data; destruct info.
+ - Intros sh. apply split_readable_share in H. destruct H as (sh1 & sh2 & H1 & H2 & H3). rewrite <- (data_at_share_join sh1 sh2 sh _ _ _).  
+    sep_apply (in_tree_split g0.1.2 ( range.1, Finite_Integer (g0.1.1.1)) lp g). sep_apply ( in_tree_split g0.2 ( Finite_Integer g0.1.1.1, range.2) rp g ). rewrite <- !sepcon_assoc. Exists sh1 sh2.  entailer!. auto.
+- entailer!. 
+Qed.
+
+
+Lemma extract_left_node_info_from_ghost_tree_rep:  forall  tg np b g_root g_current g (r_root: number * number) (range:number*number),
+   (find_ghost_set tg g_root r_root b) g_current = Some (range,np) -> ghost_tree_rep tg b g_root g r_root  |--  EX tp:val,  EX o:option ghost_info, EX lp:val, EX rp:val, 
+    node_information o range g g_current tp lp rp np  *
+   ( node_information o range g g_current tp lp rp np  -* ghost_tree_rep tg b g_root g r_root).
+Proof.
+ intros.
+revert dependent b.
+revert dependent g_root.
+revert dependent r_root.
+induction tg;intros. 
+  -  inv H. destruct r_root. destruct range. unfold ghosts.singleton in H1. Exists nullval.  Exists (@None ghost_info) nullval nullval. unfold node_information;simpl. simpl in *. entailer!.  destruct (eq_dec g_current g_root). inv H1. cancel;apply wand_refl_cancel_right. discriminate.
+  -  intros. simpl in H. unfold map_upd in H. destruct (eq_dec g_current g_root). 
+     * inv H. destruct range. simpl in *.  Intros tp sh. Exists  tp (Some ( k, v0, g0, g1)) v v1. unfold node_information. simpl in *. Exists sh. entailer!.  rewrite <- wand_sepcon_adjoint. Intro sh1. Exists tp sh1. entailer!.
+     * unfold map_add in H. destruct r_root. simpl in *. remember (find_ghost_set tg1 g0 (n0, Finite_Integer k) v g_current) as left_set. destruct left_set.
+        ** Intros rtp sh. sep_apply IHtg1. rewrite <- Heqleft_set. apply H.  Intros tp o lp rp. Exists tp o lp rp. entailer!. 
+             rewrite -> 5sepcon_assoc.  rewrite <- (emp_wand (bst_conc_nblocking_spec.atomic_ptr_at Ews rtp b * _)) . rewrite wand_sepcon_wand. apply wand_derives.
+             rewrite -> sepcon_emp;auto. Exists rtp sh. entailer!.
+        ** Intros rtp sh. sep_apply IHtg2.  Intros tp o lp rp. Exists tp o lp rp. entailer!. 
+             rewrite -> 5sepcon_assoc.  rewrite <- (emp_wand (bst_conc_nblocking_spec.atomic_ptr_at Ews rtp b * _)) . rewrite wand_sepcon_wand. apply wand_derives.
+             rewrite -> sepcon_emp;auto. Exists rtp sh. entailer!.
+
+Qed.
+
+
+Lemma extract_node_info_from_ghost_tree_rep_2:  forall  tg np b g_root x v g_current g (r_root: number * number) n n0, 
+  (find_ghost_set tg g_root r_root b) g_current = Some (n,n0,np)-> (forall k, In_ghost k tg -> check_key_exist' k r_root = true) -> sorted_ghost_tree tg-> ghost_tree_rep tg b g_root g r_root  |--  EX tp:val,  EX o:option ghost_info, EX lp:val, EX rp:val, 
+     !!(range_inclusion (n,n0) r_root = true ) && node_information o (n, n0) g g_current tp lp rp np  *
+      (( node_information o (n, n0) g g_current tp lp rp np  -* ghost_tree_rep tg b g_root g r_root)
+    && (ALL g1 g2:gname,ALL tp1:val, ( !!(o = None /\ tp = nullval  /\ (check_key_exist' x (n,n0) = true) ) && node_information (Some (x,v,g1,g2)) (n, n0) g g_current tp1 lp rp np * node_information None (n, Finite_Integer x) g g1 nullval nullval nullval lp * node_information None (Finite_Integer x, n0) g g2 nullval nullval nullval rp)  -* (!! IsEmptyGhostNode (n,n0,o) tg r_root &&ghost_tree_rep (insert_ghost x v tg g1 lp g2 rp ) b g_root g r_root))
+    && (ALL g1 g2:gname, ALL (v0:val), ( !!(o = Some(x,v0,g1,g2) /\ (check_key_exist' x (n,n0) = true)) && node_information (Some (x,v,g1,g2)) (n, n0) g g_current tp lp rp np  ) -* ( !! In_ghost x tg &&ghost_tree_rep (insert_ghost x v tg g1 lp g2 rp ) b g_root g r_root)) ).
+Proof.
+intros. 
+revert dependent r_root. 
+revert dependent b.
+revert dependent g_root.
+induction tg.
+ - intros. destruct r_root. simpl in H. unfold ghosts.singleton in H.  destruct (eq_dec g_current g_root). inv H. Exists nullval (@None ghost_info) nullval nullval. unfold node_information at 1, node_data at 1. simpl. entailer!.
+  { rewrite less_than_equal_itself. rewrite less_than_equal_itself. repeat (split;auto). } repeat apply andp_right.
+    * unfold node_information, node_data;simpl. entailer!.  apply wand_refl_cancel_right.
+    *  apply allp_right; intro g1. apply allp_right;intro g2. apply allp_right;intro tp1.  rewrite <- wand_sepcon_adjoint. unfold node_information, node_data;simpl. Intro sh.  rewrite <-!sepcon_assoc. Exists tp1 sh. cancel. entailer!. apply InEmptyGhostTree;auto.
+    *  apply allp_right; intro g1. apply allp_right;intro g2. apply allp_right;intro v0.  rewrite <- wand_sepcon_adjoint. Intros. 
+    * discriminate.
+ - intros.  simpl in H. unfold map_upd in H. destruct (eq_dec g_current g_root) eqn: Eqn.
+   * inv H. simpl. Intros tp sh.  Exists  tp (Some (k, v1, g0, g1)) v0 v2.  unfold node_information at 1, node_data at 1. Exists sh. entailer!. repeat rewrite less_than_equal_itself. simpl;auto. cancel.  repeat  apply andp_right.
+     +   rewrite <- wand_sepcon_adjoint. unfold node_information, node_data. simpl.  Intro sh1. Exists  tp sh1. entailer!.
+     + apply allp_right; intro g2. apply allp_right;intro g3. apply allp_right;intro tp1. rewrite <- wand_sepcon_adjoint. Intros a.
+     + apply allp_right; intro g2. apply allp_right;intro g3. apply allp_right;intro vp. rewrite <- wand_sepcon_adjoint. assert_PROP (Some (k, v1, g0, g1) = Some (x, vp, g2, g3)). { entailer!. } inv H4;subst. simpl.
+      destruct (x <? x) eqn: E1. apply Z.ltb_lt in E1. omega. simpl. unfold node_information, node_data. Intro sh1.  entailer!. apply InRoot_ghost. auto. Exists tp sh1. simpl. entailer!.
+ * unfold map_add in H. rename n1 into eq. destruct r_root as [n1 n2]. simpl in H. remember (find_ghost_set tg1 g0 (n1, Finite_Integer k) v0 g_current) as left_set. destruct left_set.  rename g2 into g_left.
+    ** simpl.  Intros tp sh. destruct (x <? k) eqn: E1.
+        + simpl. inv H1.  sep_apply IHtg1. rewrite <- Heqleft_set;apply H.
+         {  intros. assert (check_key_exist' k0 (n1, n2) = true). { apply H0. apply InLeft_ghost. apply H1. } unfold check_key_exist' in * . apply andb_prop in H3. destruct H3.
+             unfold gt_ghost in H13. apply H13 in H1. rewrite H3;simpl. apply Zaux.Zlt_bool_true. omega. }
+             rewrite sepcon_comm. Intros  tp0 o lp rp. Exists tp0 o lp rp. entailer!. 
+            { simpl in H1.  apply andb_prop in H1. destruct H1. assert (check_key_exist' k (n1, n2) = true). { apply H0. apply InRoot_ghost. auto. } unfold check_key_exist' in H6.  apply andb_prop in H6. destruct H6. rewrite H1;simpl. apply less_than_to_less_than_equal in H8. apply less_than_equal_transitivity with (b := (Finite_Integer k) ). apply H5. apply H8. }
+             rewrite distrib_sepcon_andp.  rewrite distrib_sepcon_andp.  repeat apply andp_derives.
+          ++ rewrite <- ( emp_wand (bst_conc_nblocking_spec.atomic_ptr_at Ews tp b * _ * _ * _ * _* _)). rewrite wand_sepcon_wand. apply wand_derives. cancel. Exists tp sh. entailer!.
+          ++ apply allp_right; intro g2. apply allp_right;intro g3. apply allp_right;intro tp1. repeat (rewrite allp_sepcon2; eapply allp_left). instantiate(1:= g3).  instantiate(1:= g2).  instantiate(1:= tp1).  rewrite <- ( emp_wand (bst_conc_nblocking_spec.atomic_ptr_at Ews tp b * _ * _ * _ * _* _)).
+             rewrite wand_sepcon_wand. apply wand_derives. cancel. simpl. Exists tp sh. entailer!. apply InLeftGhostSubTree. apply H5.
+          ++ apply allp_right; intro g2. apply allp_right;intro g3. apply allp_right;intro v5. repeat (rewrite allp_sepcon2; eapply allp_left). instantiate(1:= g3).  instantiate(1:= g2).  instantiate(1:= v5).  rewrite <- ( emp_wand (bst_conc_nblocking_spec.atomic_ptr_at Ews tp b * _ * _ * _ * _* _)).
+             rewrite wand_sepcon_wand. apply wand_derives. cancel. simpl. Exists tp sh. entailer!. apply InLeft_ghost. apply H5. 
+       +  simpl. inv H1. sep_apply IHtg1.  rewrite <- Heqleft_set;apply H.
+            { intros. assert (check_key_exist' k0 (n1, n2) = true). { apply H0. apply InLeft_ghost. apply H1. } unfold check_key_exist' in * . apply andb_prop in H3. destruct H3.
+             unfold gt_ghost in H13. apply H13 in H1. rewrite H3;simpl. apply Zaux.Zlt_bool_true. omega. }  
+         Intros tp0 o lp rp. Exists  tp0 o lp rp. entailer!.
+         { simpl in H1.  apply andb_prop in H1. destruct H1. assert (check_key_exist' k (n1, n2) = true). { apply H0. apply InRoot_ghost. auto. } unfold check_key_exist' in H6.  apply andb_prop in H6. destruct H6. rewrite H1;simpl. apply less_than_to_less_than_equal in H8. apply less_than_equal_transitivity with (b := (Finite_Integer k) ). apply H5. apply H8. }
+              rewrite -> 5sepcon_assoc, sepcon_comm.  rewrite distrib_sepcon_andp.  rewrite distrib_sepcon_andp.  repeat  apply andp_derives.
+         ++  rewrite <- !sepcon_assoc. rewrite <- ( emp_wand (bst_conc_nblocking_spec.atomic_ptr_at Ews tp b * _ * _ * _ * _* _)). rewrite wand_sepcon_wand. apply wand_derives. cancel. Exists tp sh. entailer!.
+         ++ apply allp_right; intro g2. apply allp_right;intro g3. apply allp_right;intro tp1. repeat (rewrite allp_sepcon2; eapply allp_left). instantiate(1:= g2).  instantiate(1:= g3).  instantiate(1:= tp1). 
+              rewrite <- wand_sepcon_adjoint. assert_PROP (check_key_exist' x (n,n0) = true). { simpl. entailer!. } 
+              assert (x < k). { simpl in H1. apply andb_prop in H1. apply andb_prop in H5.  destruct H1,H5. unfold less_than_equal, less_than in *. destruct n0.  apply Z.ltb_lt in H8. apply Zle_bool_imp_le in H6. omega. discriminate. discriminate.  } 
+              apply Z.ltb_nlt in E1. omega. 
+         ++ apply allp_right; intro g2. apply allp_right;intro g3. apply allp_right;intro v5. repeat (rewrite allp_sepcon2; eapply allp_left). instantiate(1:= g2).  instantiate(1:= g3).  instantiate(1:= v5). 
+              rewrite <- wand_sepcon_adjoint. assert_PROP (check_key_exist' x (n,n0) = true). { simpl. entailer!. } 
+              assert (x < k). { simpl in H1. apply andb_prop in H5. apply andb_prop in H1.  destruct H1,H5. unfold less_than_equal, less_than in *. destruct n0.  apply Z.ltb_lt in H8. apply Zle_bool_imp_le in H6. omega. discriminate. discriminate.  } 
+             apply Z.ltb_nlt in E1. omega. 
+  ** simpl. Intros tp sh. destruct (x <? k) eqn: E1.
+       + simpl. inv H1.  unfold lt_ghost in H14. sep_apply IHtg2.
+         { intros. assert (check_key_exist' k0 (n1, n2) = true). { apply H0. apply InRight_ghost. apply H1. } unfold check_key_exist' in * . apply andb_prop in H3. destruct H3.
+         apply H14 in H1. rewrite H4;simpl. rewrite andb_comm;simpl. apply Zaux.Zlt_bool_true. omega. }       
+       Intros tp0 o lp rp. Exists tp0 o lp rp. entailer!. 
+         { simpl in H1.  apply andb_prop in H1. destruct H1. assert (check_key_exist' k (n1, n2) = true). { apply H0. apply InRoot_ghost. auto. } unfold check_key_exist' in H6.  apply andb_prop in H6. destruct H6. rewrite H5;simpl. rewrite andb_comm;simpl. apply less_than_to_less_than_equal in H6. apply less_than_equal_transitivity with (b := (Finite_Integer k) ). apply H6. apply H1. }
+          rewrite -> 5sepcon_assoc, sepcon_comm.  rewrite distrib_sepcon_andp.  rewrite distrib_sepcon_andp.  repeat  apply andp_derives.
+         ++  rewrite <- !sepcon_assoc. rewrite <- ( emp_wand (bst_conc_nblocking_spec.atomic_ptr_at Ews tp b * _ * _ * _ * _* _)). rewrite wand_sepcon_wand. apply wand_derives. cancel. Exists tp sh. entailer!.
+         ++ apply allp_right; intro g2. apply allp_right;intro g3. apply allp_right;intro tp1. repeat (rewrite allp_sepcon2; eapply allp_left). instantiate(1:= g2).  instantiate(1:= g3). instantiate(1:= tp1). 
+              rewrite <- wand_sepcon_adjoint. assert_PROP (check_key_exist' x (n,n0) = true). { simpl. entailer!. } 
+              assert (k < x). { simpl in H1. apply andb_prop in H5. apply andb_prop in H1.  destruct H1,H5. unfold less_than_equal, less_than in *. destruct n.  apply Zle_bool_imp_le in H1. apply Z.ltb_lt in H5. omega. discriminate. discriminate.  } 
+             apply Z.ltb_lt in E1. omega. 
+         ++ apply allp_right; intro g2. apply allp_right;intro g3. apply allp_right;intro v3. repeat (rewrite allp_sepcon2; eapply allp_left). instantiate(1:= g2).  instantiate(1:= g3). instantiate(1:= v3). 
+              rewrite <- wand_sepcon_adjoint. assert_PROP (check_key_exist' x (n,n0) = true). { simpl. entailer!. }  
+              assert (k < x). { simpl in H1. apply andb_prop in H5. apply andb_prop in H1.  destruct H1,H5. unfold less_than_equal, less_than in *. destruct n.  apply Zle_bool_imp_le in H1. apply Z.ltb_lt in H5. omega. discriminate. discriminate.  } 
+              apply Z.ltb_lt in E1. omega. 
+        + destruct (k <? x) eqn:E2. simpl;inv H1.  
+          ++ sep_apply IHtg2.
+            {  intros. assert (check_key_exist' k0 (n1, n2) = true). { apply H0. apply InRight_ghost. apply H1. } unfold check_key_exist' in * . apply andb_prop in H3. destruct H3.
+               unfold lt_ghost in H14. apply H14 in H1. rewrite H4;simpl. rewrite andb_comm;simpl. apply Zaux.Zlt_bool_true. omega. }
+            Intros tp0 o lp rp. Exists  tp0 o lp rp. entailer!.
+            { simpl in H1.  apply andb_prop in H1. destruct H1. assert (check_key_exist' k (n1, n2) = true). { apply H0. apply InRoot_ghost. auto. } unfold check_key_exist' in H6.  apply andb_prop in H6. destruct H6. rewrite H5;simpl. rewrite andb_comm;simpl.  apply less_than_to_less_than_equal in H6. apply less_than_equal_transitivity with (b := (Finite_Integer k) ). apply H6. apply H1. }
+           rewrite -> 5sepcon_assoc, sepcon_comm.  rewrite distrib_sepcon_andp.  rewrite distrib_sepcon_andp.  repeat apply andp_derives.
+            +++  rewrite <- !sepcon_assoc.  rewrite <- ( emp_wand (bst_conc_nblocking_spec.atomic_ptr_at Ews tp b * _ * _ * _ * _* _)). rewrite wand_sepcon_wand. apply wand_derives. cancel. Exists tp sh. entailer!.
+            +++  apply allp_right; intro g2. apply allp_right;intro g3. apply allp_right;intro tp1. repeat (rewrite allp_sepcon2; eapply allp_left). instantiate(1:= g3).  instantiate(1:= g2).  instantiate(1:= tp1). rewrite <- !sepcon_assoc.   rewrite <- ( emp_wand (bst_conc_nblocking_spec.atomic_ptr_at Ews tp b * _ * _ * _ * _* _)).
+             rewrite wand_sepcon_wand. apply wand_derives. cancel. simpl. Exists tp sh. entailer!.  apply InRightGhostSubTree. apply H5. 
+            +++ apply allp_right; intro g2. apply allp_right;intro g3. apply allp_right;intro v5. repeat (rewrite allp_sepcon2; eapply allp_left). instantiate(1:= g3).  instantiate(1:= g2).  instantiate(1:= v5). rewrite <- !sepcon_assoc.  rewrite <- ( emp_wand (bst_conc_nblocking_spec.atomic_ptr_at Ews tp b * _ * _ * _ * _* _)).
+             rewrite wand_sepcon_wand. apply wand_derives. cancel. simpl. Exists tp sh. entailer!. apply InRight_ghost. apply H5. 
+         ++   inv H1.  assert (k = x ). { apply Z.ltb_nlt in E1. apply Z.ltb_nlt in E2. omega. } sep_apply IHtg2. 
+            { intros. assert (check_key_exist' k0 (n1, n2) = true). { apply H0. apply InRight_ghost. apply H3. } unfold check_key_exist' in * . apply andb_prop in H4. destruct H4.
+              unfold lt_ghost in H14. apply H14 in H3. rewrite H5;simpl. rewrite andb_comm;simpl. apply Zaux.Zlt_bool_true. omega. }
+            Intros  tp0 o lp rp. Exists  tp0 o lp rp. entailer!. 
+            { simpl in H3.  apply andb_prop in H3. destruct H3. assert (check_key_exist' x (n1, n2) = true). { apply H0. apply InRoot_ghost. auto. } unfold check_key_exist' in H6.  apply andb_prop in H6. destruct H6. rewrite H3;simpl. rewrite andb_comm;simpl. apply less_than_to_less_than_equal in H6. apply less_than_equal_transitivity with (b := (Finite_Integer x) ). apply H6. apply H1. }
+             rewrite -> 5sepcon_assoc, sepcon_comm.  rewrite distrib_sepcon_andp.  rewrite distrib_sepcon_andp.  repeat  apply andp_derives.
+            +++  rewrite <- !sepcon_assoc.  rewrite <- ( emp_wand (bst_conc_nblocking_spec.atomic_ptr_at Ews tp b * _ * _ * _ * _* _)). rewrite wand_sepcon_wand. apply wand_derives. cancel. Exists tp sh. entailer!.
+            +++ apply allp_right; intro g2. apply allp_right;intro g3. apply allp_right;intro tp1. repeat (rewrite allp_sepcon2; eapply allp_left). instantiate(1:= g2).  instantiate(1:= g3).  instantiate(1:= tp1). 
+                   rewrite <- wand_sepcon_adjoint. assert_PROP (check_key_exist' x (n,n0) = true). { simpl. entailer!. } 
+                   simpl in H2.  apply andb_prop in H3. apply andb_prop in H1.  destruct H3, H1. destruct n. simpl in H1. apply Z.ltb_lt in H1. apply Zle_bool_imp_le in H3. omega. discriminate. simpl in H1. discriminate. 
+        
+            +++ apply allp_right; intro g2. apply allp_right;intro g3. apply allp_right;intro v3. repeat (rewrite allp_sepcon2; eapply allp_left). instantiate(1:= g2).  instantiate(1:= g3).  instantiate(1:= v3). 
+                  rewrite <- wand_sepcon_adjoint. assert_PROP (check_key_exist' x (n, n0) = true). { simpl. entailer!. } 
+                 simpl in H3.  apply andb_prop in H3. apply andb_prop in H1.  destruct H3, H1. destruct n. simpl in H1. apply Z.ltb_lt in H1. apply Zle_bool_imp_le in H3. omega. discriminate. simpl in H1. discriminate.     
+
+ Qed.
+
+Lemma node_data_valid_pointer:
+  forall (info: option ghost_info) g  tp lp rp (range:number *number), node_data info g tp lp rp range |-- valid_pointer tp.
+Proof.
+  intros; unfold node_data; destruct info.
+  Intros sh; entailer!. entailer!.
+Qed.
+Hint Resolve node_data_valid_pointer : valid_pointer.
+
+Lemma node_data_saturate_local:
+  forall (info: option ghost_info) g  tp lp rp (range:number *number), node_data info g tp lp rp range  |-- !! is_pointer_or_null tp.
+Proof.
+  intros. unfold node_data; destruct info. Intros sh. entailer!. entailer!.
+Qed.
+Hint Resolve node_data_saturate_local: saturate_local.
+
+Lemma node_data_R: forall (info: option ghost_info) g  tp lp rp (range:number *number),  node_data info g tp lp rp range |-- if (eq_dec tp nullval) then !!(info = None) && emp  else 
+EX data, EX sh, !!(readable_share sh/\ info = Some data) &&  data_at sh t_struct_tree (Vint (Int.repr data.1.1.1),(data.1.1.2,(lp,rp))) tp * in_tree data.1.2( fst range, Finite_Integer data.1.1.1) lp g * in_tree data.2 ( Finite_Integer data.1.1.1, snd range) rp g.
+Proof.
+intros. unfold node_data.
+destruct info.
+- Intros sh.  assert_PROP (tp <> nullval).  { entailer!. } destruct (eq_dec tp nullval). contradiction. Exists g0 sh. entailer!.
+- Intros. destruct (eq_dec tp nullval). entailer!. contradiction.
+Qed.
+
+Lemma ghost_master1_alloc : forall r:node_info,
+  emp |-- (|==> (EX g, ghost_master1 r g))%I.
+Proof.
+ intros.
+ unfold ghost_master1, ghost_master.
+ iIntros "e".
+  iMod (own_alloc (RA := snap_PCM) (Tsh,r) compcert_rmaps.RML.R.NoneP with "e") as (g) "p".
+ simpl;auto.
+ iModIntro.
+ iExists g.
+ iFrame. 
+Qed.
   End Specifications.
 
   
